Update reachabilityTheory
New definition of close_spt

compiler/backend/reachabilityScript.sml
@@ -109,7 +109,8 @@ val delete_fail = Q.store_thm ("delete_fail",
 );
 
 val size_delete = Q.store_thm ( "size_delete",
-    `∀ n t . (size (delete n t) = if (lookup n t = NONE) then (size t) else (size t - 1))`,
+    `∀ n t . (size (delete n t) = 
+        if (lookup n t = NONE) then (size t) else (size t - 1))`,
     rw[size_def] >>
     fs[lookup_NONE_domain] >>
     TRY (qpat_assum `n NOTIN d` (qspecl_then [] mp_tac)) >>
@@ -146,21 +147,31 @@ val subspt_delete = Q.store_thm("subspt_delete",
 (**************************************** INTERSECTION LEMMAS ****************************************)
 
 val inter_union_empty = Q.store_thm("inter_union_empty",
-    `∀ a b c . isEmpty (inter (union a b) c) ⇔ isEmpty (inter a c) ∧ isEmpty (inter b c)`,
-    rw[] >> EQ_TAC >> rw[] >> `wf (inter (union a b) c) ∧ wf (inter a c)` by metis_tac[wf_inter] >>
-    fs[domain_empty] >> fs[EXTENSION] >> rw[] >> pop_assum (qspec_then `x` mp_tac) >> fs[domain_lookup] >>
-    rw[] >> fs[lookup_inter, lookup_union] >> TRY(first_x_assum (qspec_then `x` mp_tac)) >> rw[] >>
+    `∀ a b c . isEmpty (inter (union a b) c) 
+  ⇔ isEmpty (inter a c) ∧ isEmpty (inter b c)`,
+    rw[] >> EQ_TAC >> rw[] >> 
+    `wf (inter (union a b) c) ∧ wf (inter a c)` by metis_tac[wf_inter] >>
+    fs[domain_empty] >> fs[EXTENSION] >> rw[] >> 
+    pop_assum (qspec_then `x` mp_tac) >> fs[domain_lookup] >>
+    rw[] >> fs[lookup_inter, lookup_union] >> 
+    TRY(first_x_assum (qspec_then `x` mp_tac)) >> rw[] >>
     fs[lookup_inter, lookup_union] >> EVERY_CASE_TAC >> fs[]
 );
 
 val inter_insert_empty = Q.store_thm("inter_insert_empty",
-    `∀ n t1 t2 . isEmpty (inter (insert n () t1) t2) ⇒ n ∉ domain t2 ∧ isEmpty(inter t1 t2)`,
-    rw[] >> `∀ k . lookup k (inter (insert n () t1) t2) = NONE` by fs[lookup_def]
-    >- (fs[domain_lookup] >> rw[] >> fs[lookup_inter] >> pop_assum (qspec_then `n` mp_tac) >>
+    `∀ n t1 t2 . isEmpty (inter (insert n () t1) t2) 
+  ⇒ n ∉ domain t2 ∧ isEmpty(inter t1 t2)`,
+    rw[] >> 
+    `∀ k . lookup k (inter (insert n () t1) t2) = NONE` by fs[lookup_def]
+    >- (fs[domain_lookup] >> rw[] >> fs[lookup_inter] >> 
+        pop_assum (qspec_then `n` mp_tac) >>
         rw[] >> fs[] >> EVERY_CASE_TAC >> fs[])
-    >- (`wf (inter t1 t2)` by metis_tac[wf_inter] >> fs[domain_empty] >> fs[EXTENSION] >> rw[] >>
-        pop_assum (qspec_then `x` mp_tac) >> rw[] >> first_x_assum (qspec_then `x` mp_tac) >> rw[] >>
-        fs[domain_lookup, lookup_inter, lookup_insert] >> Cases_on `x = n` >> fs[] >>
+    >- (`wf (inter t1 t2)` by metis_tac[wf_inter] >> fs[domain_empty] >> 
+        fs[EXTENSION] >> rw[] >>
+        pop_assum (qspec_then `x` mp_tac) >> rw[] >> 
+        first_x_assum (qspec_then `x` mp_tac) >> rw[] >>
+        fs[domain_lookup, lookup_inter, lookup_insert] >> 
+        Cases_on `x = n` >> fs[] >>
         Cases_on `lookup n t2` >> fs[] >> CASE_TAC)
 );
 
@@ -170,7 +181,8 @@ val fromList2_value = Q.store_thm("fromList2_value",
     `∀ e l t n . MEM e l ⇔  ∃ n . lookup n (fromList2 l) = SOME e`,
     rw[lookup_fromList2] >> rw[lookup_fromList] >> fs[MEM_EL] >>
     EQ_TAC >> rw[]
-    >- (qexists_tac `n * 2` >> fs[] >> once_rewrite_tac [MULT_COMM] >> rw[EVEN_DOUBLE, MULT_DIV])
+    >- (qexists_tac `n * 2` >> fs[] >> once_rewrite_tac [MULT_COMM] >> 
+        rw[EVEN_DOUBLE, MULT_DIV])
     >- (qexists_tac `n DIV 2` >> fs[])
 );
 
@@ -194,55 +206,71 @@ val num_set_tree_union_def = Define `
      case t of
        | LN => BN t1 t2
        | LS a => BS t1 a t2
-       | BN t1' t2' => BN (num_set_tree_union t1 t1') (num_set_tree_union t2 t2')
-       | BS t1' a t2' => BS (num_set_tree_union t1 t1') a (num_set_tree_union t2 t2')) ∧
+       | BN t1' t2' => 
+            BN (num_set_tree_union t1 t1') (num_set_tree_union t2 t2')
+       | BS t1' a t2' => 
+        BS (num_set_tree_union t1 t1') a (num_set_tree_union t2 t2')) ∧
   (num_set_tree_union (BS t1 a t2) t =
      case t of
        | LN => BS t1 a t2
        | LS b => BS t1 (union a b) t2
-       | BN t1' t2' => BS (num_set_tree_union t1 t1') a (num_set_tree_union t2 t2')
-       | BS t1' b t2' => BS (num_set_tree_union t1 t1') (union a b) (num_set_tree_union t2 t2'))
+       | BN t1' t2' => 
+            BS (num_set_tree_union t1 t1') a (num_set_tree_union t2 t2')
+       | BS t1' b t2' => 
+            BS (num_set_tree_union t1 t1') (union a b) 
+                (num_set_tree_union t2 t2'))
 `;
 
 (******** THEOREMS ********)
 
 val num_set_tree_union_empty = Q.store_thm("num_set_tree_union_empty",
     `∀ t1 t2 . isEmpty(num_set_tree_union t1 t2) ⇔ isEmpty t1 ∧ isEmpty t2`,
-    Induct >> rw[num_set_tree_union_def] >> CASE_TAC >> rw[num_set_tree_union_def]
+    Induct >> rw[num_set_tree_union_def] >> CASE_TAC >> 
+    rw[num_set_tree_union_def]
 );
 
 val wf_num_set_tree_union = Q.store_thm("wf_num_set_tree_union",
-    `∀ t1 t2 result . wf t1 ∧ wf t2 ∧ num_set_tree_union t1 t2 = result ⇒ wf result`,
-    Induct >> rw[num_set_tree_union_def, wf_def] >> rw[wf_def] >> TRY(CASE_TAC) >>
-    rw[wf_def] >> TRY(metis_tac[wf_def, num_set_tree_union_empty])
+    `∀ t1 t2 result . wf t1 ∧ wf t2 ∧ num_set_tree_union t1 t2 = result 
+  ⇒ wf result`,
+    Induct >> rw[num_set_tree_union_def, wf_def] >> rw[wf_def] >> 
+    TRY(CASE_TAC) >>
+    rw[wf_def] >> 
+    TRY(metis_tac[wf_def, num_set_tree_union_empty])
 );
 
 val domain_num_set_tree_union = Q.store_thm ("domain_num_set_tree_union",
     `∀ t1 t2 . domain (num_set_tree_union t1 t2) = domain t1 ∪ domain t2`,
     Induct >> rw[num_set_tree_union_def, domain_def] >> CASE_TAC >>
-    rw[domain_def, domain_union] >> rw[UNION_ASSOC] >> rw[UNION_COMM] >> rw[UNION_ASSOC] >>
-    rw[UNION_COMM] >> metis_tac[UNION_ASSOC, UNION_COMM, UNION_IDEMPOT]
+    rw[domain_def, domain_union] >> rw[UNION_ASSOC] >> rw[UNION_COMM] >> 
+    rw[UNION_ASSOC] >> rw[UNION_COMM] >> 
+    metis_tac[UNION_ASSOC, UNION_COMM, UNION_IDEMPOT]
 );
 
 val num_set_tree_union_sym = Q.store_thm("num_set_tree_union_sym",
-    `∀ (t1 : num_set num_map) t2 . num_set_tree_union t1 t2 = num_set_tree_union t2 t1`,
-    Induct >> rw[num_set_tree_union_def] >> Cases_on `t2` >> fs[num_set_tree_union_def] >>
+    `∀ (t1 : num_set num_map) t2 . 
+        num_set_tree_union t1 t2 = num_set_tree_union t2 t1`,
+    Induct >> rw[num_set_tree_union_def] >> 
+    Cases_on `t2` >> fs[num_set_tree_union_def] >>
     fs[union_num_set_sym]
 );
 
-val lookup_domain_num_set_tree_union = Q.store_thm("lookup_domain_num_set_tree_union",
+val lookup_domain_num_set_tree_union = Q.store_thm(
+    "lookup_domain_num_set_tree_union",
     `∀ n (t1:num_set num_map) t2 x . lookup n t1 = SOME x
-    ⇒ ∃ y . lookup n (num_set_tree_union t1 t2) = SOME y ∧ domain x ⊆ domain y`,
+  ⇒ ∃ y . lookup n (num_set_tree_union t1 t2) = SOME y ∧ domain x ⊆ domain y`,
     Induct_on `t1` >> rw[]
     >- fs[lookup_def]
-    >- (fs[lookup_def, num_set_tree_union_def] >> CASE_TAC >> fs[lookup_def, domain_union])
-    >- (fs[lookup_def, num_set_tree_union_def] >> CASE_TAC >> fs[lookup_def, domain_union] >>
-        Cases_on `EVEN n` >> fs[])
-    >- (fs[lookup_def, num_set_tree_union_def] >> CASE_TAC >> fs[lookup_def, domain_union] >>
+    >- (fs[lookup_def, num_set_tree_union_def] >> CASE_TAC >> 
+        fs[lookup_def, domain_union])
+    >- (fs[lookup_def, num_set_tree_union_def] >> CASE_TAC >> 
+        fs[lookup_def, domain_union] >> Cases_on `EVEN n` >> fs[])
+    >- (fs[lookup_def, num_set_tree_union_def] >> CASE_TAC >> 
+        fs[lookup_def, domain_union] >>
         Cases_on `n = 0` >> fs[domain_union] >> Cases_on `EVEN n` >> fs[])
 );
 
-val lookup_NONE_num_set_tree_union = Q.store_thm ("lookup_NONE_num_set_tree_union",
+val lookup_NONE_num_set_tree_union = Q.store_thm (
+    "lookup_NONE_num_set_tree_union",
     `∀ n (t1:num_set num_map) t2 . lookup n t1 = NONE
     ⇒ lookup n (num_set_tree_union t1 t2) = lookup n t2`,
     Induct_on `t1` >> rw[] >> fs[lookup_def, num_set_tree_union_def] >>
@@ -250,9 +278,11 @@ val lookup_NONE_num_set_tree_union = Q.store_thm ("lookup_NONE_num_set_tree_unio
     Cases_on `EVEN n` >> fs[]
 );
 
-val lookup_SOME_SOME_num_set_tree_union = Q.store_thm ("lookup_SOME_SOME_num_set_tree_union",
-    `∀ n (t1:num_set num_map) x1 t2 x2 . lookup n t1 = SOME x1 ∧ lookup n t2 = SOME x2
-    ⇒ lookup n (num_set_tree_union t1 t2) = SOME (union x1 x2)`,
+val lookup_SOME_SOME_num_set_tree_union = Q.store_thm (
+    "lookup_SOME_SOME_num_set_tree_union",
+    `∀ n (t1:num_set num_map) x1 t2 x2 .
+    lookup n t1 = SOME x1 ∧ lookup n t2 = SOME x2
+  ⇒ lookup n (num_set_tree_union t1 t2) = SOME (union x1 x2)`,
     Induct_on `t1` >> rw[] >> fs[lookup_def, num_set_tree_union_def] >>
     Cases_on `t2` >> fs[lookup_def] >>
     Cases_on `EVEN n` >> fs[] >>
@@ -279,7 +309,8 @@ val lookup_num_set_tree_union = Q.store_thm("lookup_num_set_tree_union",
 (**************************************** CODEANALYSIS_UNION ****************************************)
 
 val codeAnalysis_union_def = Define `
-    codeAnalysis_union (r1, t1) (r2, t2) = ((union r1 r2), (num_set_tree_union t1 t2))
+    codeAnalysis_union (r1, t1) (r2, t2) = 
+        ((union r1 r2), (num_set_tree_union t1 t2))
 `
 
 (******** THEOREMS ********)
@@ -291,16 +322,19 @@ val wf_codeAnalysis_union = Q.store_thm("wf_codeAnalysis_union",
 );
 
 val wf_codeAnalysis_union_strong = Q.store_thm("wf_codeAnalysis_union_strong",
-    `∀ r3:num_set r2 r1 (t1:num_set num_map) t2 t3. wf r1 ∧ wf r2 ∧ wf t1 ∧ wf t2
-        ∧ codeAnalysis_union (r1, t1) (r2, t2) = (r3, t3) ⇒  wf r3 ∧ wf t3`,
-    rw[codeAnalysis_union_def] >> rw[wf_union] >> imp_res_tac wf_num_set_tree_union >> fs[]
+    `∀ r3:num_set r2 r1 (t1:num_set num_map) t2 t3. 
+        wf r1 ∧ wf r2 ∧ wf t1 ∧ wf t2 ∧ 
+        codeAnalysis_union (r1, t1) (r2, t2) = (r3, t3) ⇒  wf r3 ∧ wf t3`,
+    rw[codeAnalysis_union_def] >> rw[wf_union] >> 
+    imp_res_tac wf_num_set_tree_union >> fs[]
 );
 
 val domain_codeAnalysis_union = Q.store_thm("domain_codeAnalysis_union",
-    `∀ r1:num_set r2 r3 (t1:num_set num_map) t2 t3 . domain r1 ⊆ domain t1 ∧ domain r2 ⊆ domain t2 ∧
+    `∀ r1:num_set r2 r3 (t1:num_set num_map) t2 t3 . 
+    domain r1 ⊆ domain t1 ∧ domain r2 ⊆ domain t2 ∧
     codeAnalysis_union (r1, t1) (r2, t2) = (r3, t3) ⇒ domain r3 ⊆ domain t3`,
-    rw[codeAnalysis_union_def] >> rw[domain_union] >> rw[domain_num_set_tree_union] >>
-    fs[SUBSET_DEF]
+    rw[codeAnalysis_union_def] >> rw[domain_union] >> 
+    rw[domain_num_set_tree_union] >> fs[SUBSET_DEF]
 );
 
 (**************************************** SUPERDOMAIN ****************************************)
@@ -309,7 +343,8 @@ val superdomain_def = Define `
     superdomain LN = LN ∧
     superdomain (LS (t:num_set)) = t ∧
     superdomain (BN t1 t2) = union (superdomain t1) (superdomain t2) ∧
-    superdomain (BS t1 a t2) = union (superdomain t1) (union a (superdomain t2))
+    superdomain (BS t1 a t2) = 
+        union (superdomain t1) (union a (superdomain t2))
 `
 
 (* TODO - USE THIS FOLD DEFINITION OF SUPERDOMAIN
@@ -341,7 +376,8 @@ val subspt_superdomain = Q.store_thm("subspt_superdomain",
 );
 
 val superdomain_thm = Q.store_thm("superdomain_thm",
-    `∀ x y (tree:num_set num_map) . lookup x tree = SOME y ⇒ domain y ⊆ domain (superdomain tree)`,
+    `∀ x y (tree:num_set num_map) . lookup x tree = SOME y 
+  ⇒ domain y ⊆ domain (superdomain tree)`,
     Induct_on `tree` >- rw[lookup_def]
     >- rw[lookup_def, superdomain_def, foldi_def, domain_map]
     >> rw[] >> fs[lookup_def] >> Cases_on `EVEN x` >> res_tac >>
@@ -352,18 +388,24 @@ val superdomain_thm = Q.store_thm("superdomain_thm",
 val superdomain_inverse_thm = Q.store_thm("superdomain_inverse_thm",
     `∀ n tree . n ∈ domain (superdomain tree)
     ⇒ ∃ k aSet . lookup k tree = SOME aSet ∧ n ∈ domain aSet`,
-    Induct_on `tree` >> rw[superdomain_def] >> fs[lookup_def, domain_union] >> res_tac
-    >- (qexists_tac `2 * k + 2` >> fs[EVEN_DOUBLE, EVEN_ADD] >> once_rewrite_tac[MULT_COMM] >> fs[DIV_MULT])
-    >- (qexists_tac `2 * k + 1` >> fs[EVEN_DOUBLE, EVEN_ADD] >> once_rewrite_tac[MULT_COMM] >> fs[MULT_DIV])
-    >- (qexists_tac `2 * k + 2` >> fs[EVEN_DOUBLE, EVEN_ADD] >> once_rewrite_tac[MULT_COMM] >> fs[DIV_MULT])
+    Induct_on `tree` >> rw[superdomain_def] >> 
+    fs[lookup_def, domain_union] >> res_tac
+    >- (qexists_tac `2 * k + 2` >> fs[EVEN_DOUBLE, EVEN_ADD] >> 
+        once_rewrite_tac[MULT_COMM] >> fs[DIV_MULT])
+    >- (qexists_tac `2 * k + 1` >> fs[EVEN_DOUBLE, EVEN_ADD] >> 
+        once_rewrite_tac[MULT_COMM] >> fs[MULT_DIV])
+    >- (qexists_tac `2 * k + 2` >> fs[EVEN_DOUBLE, EVEN_ADD] >> 
+        once_rewrite_tac[MULT_COMM] >> fs[DIV_MULT])
     >- (qexists_tac `0` >> fs[])
-    >- (qexists_tac `2 * k + 1` >> fs[EVEN_DOUBLE, EVEN_ADD] >> once_rewrite_tac[MULT_COMM] >> fs[MULT_DIV])
+    >- (qexists_tac `2 * k + 1` >> fs[EVEN_DOUBLE, EVEN_ADD] >> 
+        once_rewrite_tac[MULT_COMM] >> fs[MULT_DIV])
 );
 
 val superdomain_not_in_thm = Q.store_thm("superdomain_not_in_thm",
-    `∀ n tree . n ∉ domain (superdomain tree) ⇒ ∀ k aSet . lookup k tree = SOME aSet ⇒ n ∉ domain aSet`,
-    Induct_on `tree` >> rw[superdomain_def] >> fs[lookup_def, domain_union] >> res_tac >>
-    Cases_on `k = 0` >> Cases_on `EVEN k` >> fs[] >> metis_tac[]
+    `∀ n tree . n ∉ domain (superdomain tree) 
+  ⇒ ∀ k aSet . lookup k tree = SOME aSet ⇒ n ∉ domain aSet`,
+    Induct_on `tree` >> rw[superdomain_def] >> fs[lookup_def, domain_union] >> 
+    res_tac >> Cases_on `k = 0` >> Cases_on `EVEN k` >> fs[] >> metis_tac[]
 );
 
 (*********************************** WF_SET_TREE/MAKE WF_SET_TREE ***********************************)
@@ -384,18 +426,21 @@ val mk_wf_set_tree_def = Define `
 
 val mk_wf_set_tree_domain = Q.store_thm("mk_wf_set_tree_domain",
     `∀ tree . domain tree ⊆ domain (mk_wf_set_tree tree)`,
-    Induct >> rw[mk_wf_set_tree_def, domain_map, domain_mk_wf, domain_union, SUBSET_DEF]
+    Induct >> 
+    rw[mk_wf_set_tree_def, domain_map, domain_mk_wf, domain_union, SUBSET_DEF]
 );
 
 val mk_wf_set_tree_thm = Q.store_thm("mk_wf_set_tree_thm",
     `∀ x tree . x = mk_wf_set_tree tree ⇒ wf_set_tree x`,
-    rw[mk_wf_set_tree_def, wf_set_tree_def] >> fs[lookup_map] >> rw[domain_map, domain_union] >>
-    fs[lookup_union] >> Cases_on `lookup x' tree` >> fs[] >- fs[lookup_map] >> rw[] >>
+    rw[mk_wf_set_tree_def, wf_set_tree_def] >> fs[lookup_map] >> 
+    rw[domain_map, domain_union] >> fs[lookup_union] >> 
+    Cases_on `lookup x' tree` >> fs[] >- fs[lookup_map] >> rw[] >> 
     qspecl_then [`x'`, `x`, `tree`] mp_tac superdomain_thm >> rw[SUBSET_DEF]
 );
 
 val lookup_mk_wf_set_tree = Q.store_thm("lookup_mk_wf_set_tree",
-    `∀ n tree x . lookup n tree = SOME x ⇒ ∃ y . lookup n (mk_wf_set_tree tree) = SOME y ∧ domain x = domain y`,
+    `∀ n tree x . lookup n tree = SOME x 
+  ⇒ ∃ y . lookup n (mk_wf_set_tree tree) = SOME y ∧ domain x = domain y`,
     rw[mk_wf_set_tree_def] >> rw[lookup_map] >> rw[lookup_union]
 );
 
@@ -427,37 +472,74 @@ val getOne_domain = Q.store_thm("getOne_domain",
 (**************************************** CLOSE_SPT/CLOSURE_SPT ****************************************)
 
 (******** CLOSE_SPT ********)
-
 val close_spt_def = tDefine "close_spt" `
-    (close_spt (reachable :num_set) (seen :num_set) tree =
-    let toLook = difference seen reachable in
-    if toLook = LN then reachable else
-    let index = (getOne toLook) in
-    case (lookup index tree) of
-        | NONE => reachable
-        | SOME new =>
-        close_spt (insert index () reachable) (union new seen) (delete index tree)
-    )`
-    (WF_REL_TAC `measure (λ (reachable, seen, tree) . size tree)`
-    \\ rw[size_delete, lookup_zero]
-    \\ imp_res_tac lookup_zero
-    \\ fs[]);
+    close_spt (reachable :num_set) (seen :num_set) (tree :num_set spt) =
+        let to_look = difference seen reachable in
+        let new_sets = inter tree to_look in
+            if new_sets = LN then reachable else
+                let new_set = spt_fold union LN new_sets in
+                    close_spt (union reachable to_look) (union seen new_set)
+                        tree
+    `
+    (
+        WF_REL_TAC `measure (λ (r, _, t) . size (difference t r))` >>
+        rw[] >>
+        match_mp_tac size_diff_less >>
+        fs[domain_union, domain_difference] >>
+        fs[inter_eq_LN, IN_DISJOINT, domain_difference] >>
+        qexists_tac `x` >>
+        fs[]
+    )
 
 val close_spt_ind = theorem "close_spt_ind";
 
+val wf_spt_fold_tree = Q.store_thm("wf_spt_fold_tree",
+    `∀ tree : num_set num_map y : num_set. 
+        wf tree ∧ (∀ n x . (lookup n tree = SOME x) ⇒ wf x) ∧ wf y
+      ⇒ wf(spt_fold union y tree)`, 
+    Induct >> rw[] >> fs[spt_fold_def]
+    >- (fs[wf_def] >> metis_tac[lookup_def, wf_union])
+    >> `wf(spt_fold union y tree)` by (
+            last_x_assum match_mp_tac >>
+            fs[] >> rw[]
+            >- fs[wf_def]
+            >> last_x_assum match_mp_tac >>
+               qexists_tac `2 * n + 2` >>
+               fs[lookup_def] >> fs[EVEN_DOUBLE, EVEN_ADD] >>
+               once_rewrite_tac[MULT_COMM] >> fs[DIV_MULT])
+    >> (last_x_assum match_mp_tac >> fs[] >> rw[] 
+        >-  fs[wf_def]
+        >- (last_x_assum match_mp_tac >> 
+            qexists_tac `2 * n + 1` >> fs[lookup_def, EVEN_DOUBLE, EVEN_ADD] >>
+            once_rewrite_tac[MULT_COMM] >> fs[MULT_DIV])
+        >>  `wf a` by (last_x_assum match_mp_tac >>
+                qexists_tac `0` >> fs[lookup_def]) >>
+            fs[wf_union])
+);
+
 val wf_close_spt = Q.store_thm("wf_close_spt",
-    `∀ reachable seen tree. (wf reachable) ∧ (wf seen) ∧ (wf tree) ∧ (∀ n x . (lookup n tree = SOME x) ⇒ wf x)
-    ⇒ wf (close_spt reachable seen tree)`,
-    recInduct close_spt_ind >> rw[] >> once_rewrite_tac [close_spt_def] >> rw[] >>
-    CASE_TAC >- rw[]
-    >> `∀n x. lookup n (delete (getOne (difference seen reachable)) tree) = SOME x ⇒ wf x` by (
-            rw[lookup_delete] >> metis_tac[] ) >>
-        metis_tac [wf_insert, wf_union, wf_delete, lookup_delete]
+    `∀ reachable seen tree. (wf reachable) ∧ (wf seen) ∧ (wf tree) ∧ 
+        (∀ n x . (lookup n tree = SOME x) ⇒ wf x)
+  ⇒ wf (close_spt reachable seen tree)`,
+    recInduct close_spt_ind >> rw[] >>
+    once_rewrite_tac [close_spt_def] >> rw[] >> 
+    fs[] >>
+    last_x_assum match_mp_tac >>
+    reverse(rw[]) >> fs[wf_union, wf_difference]
+    >-  metis_tac[] 
+    >>  match_mp_tac wf_union >>
+        fs[] >>
+        match_mp_tac wf_spt_fold_tree >>
+        fs[wf_def] >>
+        fs[lookup_inter] >>
+        rw[] >> EVERY_CASE_TAC >> fs[] >> rveq >>
+        metis_tac[]
 );
 
 (******** CLOSURE_SPT ********)
 
-val closure_spt_def = Define `closure_spt start tree = close_spt LN start tree`;
+val closure_spt_def = Define 
+    `closure_spt start tree = close_spt LN start tree`;
 
 (**************************************** ADJACENCY/REACHABILITY ****************************************)
 
@@ -465,8 +547,9 @@ val closure_spt_def = Define `closure_spt start tree = close_spt LN start tree`;
 
 val isAdjacent_def = Define `
     isAdjacent tree x y =
-    ∃ aSetx aSety. ( lookup x tree = SOME aSetx ) ∧ ( lookup y aSetx = SOME () )
-        ∧ ( lookup y tree = SOME aSety )
+    ∃ aSetx aSety. 
+        ( lookup x tree = SOME aSetx ) ∧ ( lookup y aSetx = SOME () ) ∧ 
+        ( lookup y tree = SOME aSety )
 `;
 
 val adjacent_domain = Q.store_thm("adjacent_domain",
@@ -481,8 +564,10 @@ val isReachable_def = Define `
 `;
 
 val reachable_domain = Q.store_thm("reachable_domain",
-    `∀ tree x y . isReachable tree x y ⇒ (x = y ∨ (x ∈ domain tree ∧ y ∈ domain tree))`,
-    simp[isReachable_def] >> strip_tac >> ho_match_mp_tac RTC_INDUCT_RIGHT1 >> metis_tac[adjacent_domain]
+    `∀ tree x y . isReachable tree x y 
+  ⇒ (x = y ∨ (x ∈ domain tree ∧ y ∈ domain tree))`,
+    simp[isReachable_def] >> strip_tac >> ho_match_mp_tac RTC_INDUCT_RIGHT1 >> 
+    metis_tac[adjacent_domain]
 );
 
 val rtc_isAdjacent = Q.store_thm("rtc_isAdjacent",
@@ -498,52 +583,74 @@ val rtc_isAdjacent = Q.store_thm("rtc_isAdjacent",
 
 (******** SUPERDOMAIN/NUM_SET_TREE_UNION ********)
 
-val domain_superdomain_num_set_tree_union = Q.store_thm("domain_superdomain_num_set_tree_union",
-    `∀ t1 t2 . domain (superdomain t1) ⊆ domain (superdomain (num_set_tree_union t1 t2))`,
+val domain_superdomain_num_set_tree_union = Q.store_thm(
+    "domain_superdomain_num_set_tree_union",
+    `∀ t1 t2 . domain (superdomain t1) 
+        ⊆ domain (superdomain (num_set_tree_union t1 t2))`,
     fs[SUBSET_DEF] >> rw[] >> imp_res_tac superdomain_inverse_thm >>
-    imp_res_tac lookup_domain_num_set_tree_union >> pop_assum (qspec_then `t2` mp_tac) >>
+    imp_res_tac lookup_domain_num_set_tree_union >> 
+    pop_assum (qspec_then `t2` mp_tac) >>
     rw[] >> imp_res_tac superdomain_thm >> metis_tac[SUBSET_DEF]
 );
 
-val domain_superdomain_num_set_tree_union_STRONG = Q.store_thm("domain_superdomain_num_set_tree_union_STRONG",
-    `∀ t1 t2 . domain (superdomain t1) ∪ domain (superdomain t2) = domain (superdomain (num_set_tree_union t1 t2))`,
+val domain_superdomain_num_set_tree_union_STRONG = Q.store_thm(
+    "domain_superdomain_num_set_tree_union_STRONG",
+    `∀ t1 t2 . domain (superdomain t1) ∪ domain (superdomain t2) = 
+        domain (superdomain (num_set_tree_union t1 t2))`,
     fs[EXTENSION] >> rw[] >> EQ_TAC >> rw[]
-    >- metis_tac[domain_superdomain_num_set_tree_union, SUBSET_DEF, num_set_tree_union_sym]
-    >- metis_tac[domain_superdomain_num_set_tree_union, SUBSET_DEF, num_set_tree_union_sym]
-    >- (imp_res_tac superdomain_inverse_thm >> fs[lookup_num_set_tree_union] >> EVERY_CASE_TAC >> fs[]
+    >- metis_tac[domain_superdomain_num_set_tree_union, 
+                 SUBSET_DEF, num_set_tree_union_sym]
+    >- metis_tac[domain_superdomain_num_set_tree_union, 
+                 SUBSET_DEF, num_set_tree_union_sym]
+    >- (imp_res_tac superdomain_inverse_thm >> fs[lookup_num_set_tree_union] >>
+        EVERY_CASE_TAC >> fs[]
         >- (disj1_tac >> imp_res_tac superdomain_thm >> fs[SUBSET_DEF])
         >- (disj2_tac >> imp_res_tac superdomain_thm >> fs[SUBSET_DEF])
-        >- (rveq >> imp_res_tac superdomain_thm >> fs[SUBSET_DEF, domain_union]))
+        >- (rveq >> imp_res_tac superdomain_thm >> 
+            fs[SUBSET_DEF, domain_union])
+       )
 );
 
 (******** MK_WF_SET_TREE/NUM_SET_TREE_UNION ********)
 
-val mk_wf_set_tree_num_set_tree_union = Q.store_thm("mk_wf_set_tree_num_set_tree_union",
+val mk_wf_set_tree_num_set_tree_union = Q.store_thm(
+    "mk_wf_set_tree_num_set_tree_union",
     `∀ t1 t2 . mk_wf_set_tree (num_set_tree_union t1 t2) =
         num_set_tree_union (mk_wf_set_tree t1) (mk_wf_set_tree t2)`,
     rw[] >>
-    `wf (mk_wf_set_tree (num_set_tree_union t1 t2))` by metis_tac[mk_wf_set_tree_thm, wf_set_tree_def] >>
+    `wf (mk_wf_set_tree (num_set_tree_union t1 t2))` 
+        by metis_tac[mk_wf_set_tree_thm, wf_set_tree_def] >>
     `wf (num_set_tree_union (mk_wf_set_tree t1) (mk_wf_set_tree t2))` by
-        metis_tac[mk_wf_set_tree_thm, wf_set_tree_def, wf_num_set_tree_union] >>
-    rw[spt_eq_thm] >> simp[mk_wf_set_tree_def] >> fs[lookup_map] >> fs[lookup_union] >> fs[lookup_map] >>
-    fs[lookup_num_set_tree_union] >> fs[lookup_map] >> fs[lookup_union] >> fs[lookup_map] >>
-    fs[OPTION_MAP_COMPOSE, mk_wf_def] >> Cases_on `lookup n t1` >> Cases_on `lookup n t2` >> fs[] >>
-    EVERY_CASE_TAC >> fs[mk_wf_def, union_def] >> fs[lookup_NONE_domain, GSYM domain_lookup] >>
-    qspecl_then [`t1`, `t2`] mp_tac domain_superdomain_num_set_tree_union_STRONG >> strip_tac >>
-    fs[EXTENSION]
+        metis_tac[mk_wf_set_tree_thm, wf_set_tree_def, 
+                  wf_num_set_tree_union] >>
+    rw[spt_eq_thm] >> simp[mk_wf_set_tree_def] >> fs[lookup_map] >> 
+    fs[lookup_union] >> fs[lookup_map] >>
+    fs[lookup_num_set_tree_union] >> fs[lookup_map] >> 
+    fs[lookup_union] >> fs[lookup_map] >>
+    fs[OPTION_MAP_COMPOSE, mk_wf_def] >> Cases_on `lookup n t1` >> 
+    Cases_on `lookup n t2` >> fs[] >>
+    EVERY_CASE_TAC >> fs[mk_wf_def, union_def] >> 
+    fs[lookup_NONE_domain, GSYM domain_lookup] >>
+    qspecl_then [`t1`, `t2`] mp_tac 
+        domain_superdomain_num_set_tree_union_STRONG >> 
+    strip_tac >> fs[EXTENSION]
     >-  metis_tac[]
-    >- (qsuff_tac `n ∈ domain (superdomain (num_set_tree_union t1 t2))` >- rw[domain_lookup]
+    >- (qsuff_tac `n ∈ domain (superdomain (num_set_tree_union t1 t2))` 
+        >- rw[domain_lookup]
         >> imp_res_tac domain_lookup >> metis_tac[])
-    >- (qsuff_tac `n ∈ domain (superdomain (num_set_tree_union t1 t2))` >- rw[domain_lookup]
+    >- (qsuff_tac `n ∈ domain (superdomain (num_set_tree_union t1 t2))` 
+        >- rw[domain_lookup]
         >> imp_res_tac domain_lookup >> metis_tac[])
-    >- (qsuff_tac `n ∈ domain (superdomain (num_set_tree_union t1 t2))` >- rw[domain_lookup]
+    >- (qsuff_tac `n ∈ domain (superdomain (num_set_tree_union t1 t2))` 
+        >- rw[domain_lookup]
         >> imp_res_tac domain_lookup >> metis_tac[])
     >-  metis_tac[mk_wf_union]
 );
 
 (******** ADJACENCY/REACHABILITY ********)
 
-val isAdjacent_num_set_tree_union = Q.store_thm("isAdjacent_num_set_tree_union",
+val isAdjacent_num_set_tree_union = Q.store_thm(
+    "isAdjacent_num_set_tree_union",
     `∀ t1 t2 n m .
         isAdjacent t1 n m ⇒ isAdjacent (num_set_tree_union t1 t2) n m`,
     rw[isAdjacent_def] >> imp_res_tac lookup_domain_num_set_tree_union >>
@@ -552,21 +659,26 @@ val isAdjacent_num_set_tree_union = Q.store_thm("isAdjacent_num_set_tree_union",
     fs[SUBSET_DEF, domain_lookup]
 );
 
-val isAdjacent_wf_set_tree_num_set_tree_union = Q.store_thm ("isAdjacent_wf_set_tree_num_set_tree_union",
+val isAdjacent_wf_set_tree_num_set_tree_union = Q.store_thm (
+    "isAdjacent_wf_set_tree_num_set_tree_union",
     `∀ t1 t2 n m .
         isAdjacent (mk_wf_set_tree t1) n m
         ⇒ isAdjacent (mk_wf_set_tree (num_set_tree_union t1 t2)) n m`,
     rw[isAdjacent_def] >> fs[mk_wf_set_tree_def] >> fs[lookup_map] >>
-    fs[lookup_union] >> fs[lookup_map] >> fs[PULL_EXISTS] >> fs[lookup_num_set_tree_union] >>
+    fs[lookup_union] >> fs[lookup_map] >> fs[PULL_EXISTS] >> 
+    fs[lookup_num_set_tree_union] >>
     Cases_on `lookup n t1` >> fs[] >> Cases_on `lookup n t2` >> fs[] >>
-    rveq >> fs[lookup_def, mk_wf_def, lookup_union] >> EVERY_CASE_TAC >> fs[] >>
+    rveq >> fs[lookup_def, mk_wf_def, lookup_union] >> 
+    EVERY_CASE_TAC >> fs[] >>
     qspecl_then [`t1`, `t2`] mp_tac domain_superdomain_num_set_tree_union >>
     rw[SUBSET_DEF, domain_lookup]
 );
 
-val isReachable_wf_set_tree_num_set_tree_union = Q.store_thm ("isReachable_wf_set_tree_num_set_tree_union",
+val isReachable_wf_set_tree_num_set_tree_union = Q.store_thm (
+    "isReachable_wf_set_tree_num_set_tree_union",
     `∀ t1 t2 n m .
-        isReachable (mk_wf_set_tree t1) n m ⇒ isReachable (mk_wf_set_tree (num_set_tree_union t1 t2)) n m`,
+        isReachable (mk_wf_set_tree t1) n m 
+      ⇒ isReachable (mk_wf_set_tree (num_set_tree_union t1 t2)) n m`,
     simp[isReachable_def] >> strip_tac >> strip_tac >>
     ho_match_mp_tac RTC_INDUCT_RIGHT1 >> rw[] >>
     simp[Once RTC_CASES2] >> disj2_tac >> qexists_tac `m` >> fs[] >>
@@ -581,96 +693,295 @@ val isReachable_wf_set_tree_num_set_tree_union = Q.store_thm ("isReachable_wf_se
 
 (**************************************** CLOSE_SPT ****************************************)
 
+val lookup_spt_fold_union = Q.store_thm("lookup_spt_fold_union",
+    `∀ tree : num_set num_map y : num_set n : num .
+        lookup n (spt_fold union y tree) = SOME ()
+      ⇒ lookup n y = SOME () ∨ 
+        ∃ n1 s . lookup n1 tree = SOME s ∧ lookup n s = SOME ()`,
+    Induct >> rw[]
+    >-  fs[spt_fold_def]
+    >-  (fs[spt_fold_def, lookup_union] >> EVERY_CASE_TAC >>
+        fs[] >>
+        DISJ2_TAC >>
+        qexists_tac `0` >> qexists_tac `a` >> fs[lookup_def])
+    >- (
+        fs[spt_fold_def] >>
+        res_tac
+        >- (
+            res_tac >> fs[]
+            >- (
+               DISJ2_TAC >>
+               fs[lookup_def] >>
+               qexists_tac `n1 * 2 + 2` >> qexists_tac `s` >>
+               fs[EVEN_DOUBLE, EVEN_ADD] >>
+               once_rewrite_tac[MULT_COMM] >>
+               fs[DIV_MULT]
+               )
+            >- (
+               DISJ2_TAC >>
+               fs[lookup_def] >>
+               qexists_tac `n1' * 2 + 2` >> qexists_tac `s'` >>
+               fs[EVEN_DOUBLE, EVEN_ADD] >>
+               once_rewrite_tac[MULT_COMM] >>
+               fs[DIV_MULT]
+               )
+            )
+        >- (
+            res_tac >> fs[] >>
+            DISJ2_TAC >>
+            fs[lookup_def] >>
+            qexists_tac `2 * n1 + 1` >> qexists_tac `s` >>
+            fs[EVEN_DOUBLE, EVEN_ADD] >>
+            once_rewrite_tac[MULT_COMM] >>
+            fs[MULT_DIV]
+            )
+        )
+    >- (
+        fs[spt_fold_def] >>
+        res_tac
+        >- (
+            fs[lookup_union] >>
+            EVERY_CASE_TAC
+            >- (
+                res_tac >> fs[]
+                >- (
+                   DISJ2_TAC >>
+                   fs[lookup_def] >>
+                   qexists_tac `n1 * 2 + 2` >> qexists_tac `s` >>
+                   fs[EVEN_DOUBLE, EVEN_ADD] >>
+                   once_rewrite_tac[MULT_COMM] >>
+                   fs[DIV_MULT]
+                   )
+                >- (
+                   DISJ2_TAC >>
+                   fs[lookup_def] >>
+                   qexists_tac `n1' * 2 + 2` >> qexists_tac `s'` >>
+                   fs[EVEN_DOUBLE, EVEN_ADD] >>
+                   once_rewrite_tac[MULT_COMM] >>
+                   fs[DIV_MULT]
+                   )
+                )
+            >- (
+                DISJ2_TAC >>
+                qexists_tac `0` >> qexists_tac `a` >> 
+                fs[lookup_def]
+                )
+            )
+        >- (
+            DISJ2_TAC >>
+            fs[lookup_def] >>
+            qexists_tac `2 * n1 + 1` >> qexists_tac `s` >>
+            fs[EVEN_DOUBLE, EVEN_ADD] >>
+            once_rewrite_tac[MULT_COMM] >>
+            fs[MULT_DIV]
+            )
+    )
+);
+
+val lookup_spt_fold_union_STRONG = Q.store_thm("lookup_spt_fold_union_STRONG",
+    `∀ tree : num_set num_map y : num_set n : num .
+        lookup n (spt_fold union y tree) = SOME ()
+      <=> lookup n y = SOME () ∨ 
+        ∃ n1 s . lookup n1 tree = SOME s ∧ lookup n s = SOME ()`,
+    Induct >> rw[] >> EQ_TAC >> fs[lookup_spt_fold_union] >> rw[] >>
+    fs[spt_fold_def, lookup_def, lookup_union]
+    >- (EVERY_CASE_TAC >> fs[])
+    >- (EVERY_CASE_TAC >> fs[]
+        >- (DISJ1_TAC >> DISJ2_TAC >> 
+            qexists_tac `(n1 - 1) DIV 2` >> qexists_tac `s` >> fs[])
+        >- (DISJ2_TAC >>
+            qexists_tac `(n1 - 1) DIV 2` >> qexists_tac `s` >> fs[])
+        )
+    >- (EVERY_CASE_TAC >> fs[])
+    >- (EVERY_CASE_TAC >> fs[]
+        >- (rw[] >> fs[NOT_NONE_SOME]) 
+        >- (DISJ1_TAC >> DISJ2_TAC >>
+            qexists_tac `(n1 - 1) DIV 2` >> qexists_tac `s` >> fs[])
+        >- (DISJ2_TAC >>
+            qexists_tac `(n1 - 1) DIV 2` >> qexists_tac `s` >> fs[])
+        )
+);
+                
+val subspt_domain_spt_fold_union = Q.store_thm("subspt_domain_spt_fold_union", 
+    `∀ t1 : num_set num_map t2 y : num_set .
+        subspt t1 t2 
+      ⇒ domain (spt_fold union y t1) ⊆ domain (spt_fold union y t2)`,
+    rw[SUBSET_DEF] >> fs[domain_lookup] >> 
+    qspecl_then [`t1`, `y`] mp_tac lookup_spt_fold_union_STRONG >> 
+    qspecl_then [`t2`, `y`] mp_tac lookup_spt_fold_union_STRONG >> 
+    ntac 2 strip_tac >> res_tac 
+    >- metis_tac[]
+    >> ntac 2 (first_x_assum kall_tac) >>
+       `lookup n1 t2 = SOME s` by fs[subspt_def, domain_lookup] >> 
+       metis_tac[] 
+);
+
+val domain_spt_fold_union = Q.store_thm("domain_spt_fold_union",
+    `∀ tree : num_set num_map y : num_set .
+        (∀ k v . lookup k tree = SOME v ⇒ domain v ⊆ domain tree)
+      ⇒ domain (spt_fold union y tree) ⊆ domain y ∪ domain tree`,
+    rw[] >> qspec_then `tree` mp_tac lookup_spt_fold_union >>
+    rw[] >> fs[SUBSET_DEF, domain_lookup] >> rw[] >> res_tac >> fs[] >>
+    metis_tac[]
+);
+
+val domain_spt_fold_union_LN = Q.store_thm("domain_spt_fold_union_LN",
+    `∀ tree : num_set num_map  .
+        (∀ k v . lookup k tree = SOME v ⇒ domain v ⊆ domain tree)
+      ⇔ domain (spt_fold union LN tree) ⊆ domain tree`,
+    rw[] >> EQ_TAC >> rw[]
+    >- (drule domain_spt_fold_union >> 
+        strip_tac >> first_x_assum (qspec_then `LN` mp_tac) >> fs[])
+    >- (qspec_then `tree` mp_tac lookup_spt_fold_union_STRONG >>
+        rw[] >> fs[SUBSET_DEF, domain_lookup, lookup_def] >> rw[] >> 
+        metis_tac[])
+);
+
 val close_spt_thm = Q.store_thm("close_spt_thm",
-    `∀ reachable seen tree fullTree x (roots:num set) .
-        (wf reachable) ∧ (wf seen) ∧ (wf tree) ∧ (wf fullTree) ∧
-        (∀ n x . (lookup n fullTree = SOME x) ⇒ wf x) ∧
-        (close_spt reachable seen tree = x) ∧
+    `∀ reachable seen tree closure (roots : num set) .
+        (wf reachable) ∧ (wf seen) ∧ (wf_set_tree tree) ∧ 
+        (close_spt reachable seen tree = closure) ∧
         (subspt reachable seen) ∧
-        (subspt tree fullTree) ∧
-        (∀ n . n ∉ domain (reachable) ⇒ (lookup n tree = lookup n fullTree)) ∧
-        (∀ k . k ∈ domain (seen) ⇒ (∃ n . (n ∈ roots) ∧ (isReachable fullTree n k))) ∧
-        (∀ k . k ∈ domain (reachable) ⇒ (∀ a . (isAdjacent fullTree k a) ⇒ a ∈ domain (seen))) ∧
         (roots ⊆ domain (seen)) ∧
-        (roots ⊆ domain (fullTree)) ∧
-        (wf_set_tree fullTree)
-      ⇒ (domain x = {a | ∃ n . (isReachable fullTree n a) ∧ (n ∈ roots)})`,
-    recInduct close_spt_ind
-    >> rw[] >> once_rewrite_tac [close_spt_def] >> simp[]
-    >> IF_CASES_TAC
+        (domain seen ⊆ domain tree) ∧ 
+        (∀ k . k ∈ domain (seen) 
+            ⇒ (∃ n . (n ∈ roots) ∧ (isReachable tree n k))) ∧
+        (∀ k . k ∈ domain (reachable) 
+            ⇒ (∀ a . (isAdjacent tree k a) ⇒ a ∈ domain (seen)))
+      ⇒ (domain closure = {a | ∃ n . (isReachable tree n a) ∧ (n ∈ roots)})`
+  ,
+    recInduct close_spt_ind >> rw[] >> 
+    once_rewrite_tac [close_spt_def] >> simp[] >> fs[wf_set_tree_def] >>
+    IF_CASES_TAC
     >- (
-        drule empty_sub >> fs[] >> rw[] >> fs[] >> fs[EXTENSION] >> rw[] >> EQ_TAC >> rw[]
-        >- metis_tac[]
-        >> fs[SUBSET_DEF] >> fs[isReachable_def] >> `roots ⊆ domain (reachable)` by fs[SUBSET_DEF] >>
-            drule rtc_isAdjacent >> rw[] >> metis_tac[]
-       )
-    >> CASE_TAC >> fs[] >> fs[subspt_domain] >> rw[] >> fs[SUBSET_DEF] >> rw[EXTENSION]
+        imp_res_tac inter_eq_LN  >>
+        imp_res_tac subspt_domain >>
+        fs[SUBSET_DEF, EXTENSION, IN_DISJOINT, domain_difference] >>
+        `domain reachable = domain seen` by (
+            fs[EXTENSION] >> rw[] >> EQ_TAC >> fs[] >> metis_tac[]) >>
+        imp_res_tac num_set_domain_eq >>
+        fs[] >> rveq >> rw[] >> EQ_TAC >> rw[] 
+        >- (qpat_x_assum `∀ k . k ∈ domain seen ⇒ _` (qspec_then `x` mp_tac) >>
+            reverse(impl_tac) >> rw[] >> metis_tac[])
+        >> (imp_res_tac reachable_domain >> rveq >> fs[] >>
+            res_tac >>
+            qspecl_then [`domain reachable`, `domain reachable`, `tree`] mp_tac 
+                (rtc_isAdjacent |> GEN_ALL) >>
+            strip_tac >> fs[] >>
+            fs[isReachable_def] >>
+            res_tac)
+        )
     >- (
-        fs[lookup_NONE_domain] >>
-        `getOne (difference seen reachable) ∈ domain (difference seen reachable)`
-            by rw[wf_difference, getOne_domain] >>
-        fs[domain_difference] >> res_tac >> imp_res_tac reachable_domain >>
-        `n ∈ domain fullTree` by metis_tac[] >> fs[domain_lookup] >> rfs[]
-       )
-    >> rfs[EXTENSION] >> pop_assum match_mp_tac >>
-    `∀ n x. lookup n tree = SOME x ⇒ wf x` by (fs[subspt_def, domain_lookup] >> metis_tac[]) >>
-    `getOne (difference seen reachable) ∈ domain (union x seen)` by (
-        rw[domain_union, getOne_domain] >>
-        `domain (difference seen reachable) ⊆ domain seen` by rw[domain_difference] >>
-        `getOne(difference seen reachable)∈ domain(difference seen reachable)`
-            by rw[getOne_domain, wf_difference] >>
-         fs[SUBSET_DEF] >> metis_tac [] ) >>
-    `∀k. k = getOne (difference seen reachable) ∨ k ∈ domain reachable ⇒
-        ∀a. isAdjacent fullTree k a ⇒ a ∈ domain (union x seen)` by (
-        pop_assum kall_tac >> strip_tac >> Cases_on `k ∈ domain reachable`
-        >> simp[domain_union] >> metis_tac [domain_union, isAdjacent_def, domain_lookup, SOME_11]) >>
-    `∀k. k ∈ domain (union x seen) ⇒ ∃n. n ∈ roots ∧ isReachable fullTree n k` by (
-        reverse(rw[domain_union] >> Cases_on `k ∈ domain seen` >> rw[])
-        >- metis_tac []
-        >> `getOne (difference seen reachable) ∈ domain seen ∧
-            getOne (difference seen reachable) ∉ domain reachable`
-            by ( `getOne(difference seen reachable) ∈ domain (difference seen reachable)`
-                    by rw[wf_difference, getOne_domain] >>
-                 fs[domain_difference]) >>
-            res_tac >> qexists_tac `n` >> rw[isReachable_def, Once RTC_CASES2] >> disj2_tac >>
-            qexists_tac `getOne (difference seen reachable)` >> rw[isAdjacent_def]
-            >- metis_tac[isReachable_def] >> qexists_tac `x` >>
-            res_tac >> rw[] >> fs[domain_lookup] >>
-            qpat_x_assum `wf_set_tree _` assume_tac >> fs[wf_set_tree_def] >>
-            qpat_x_assum `_ = SOME x` assume_tac >> qpat_x_assum `∀ x . _` kall_tac >>
-            first_x_assum drule >> rw[SUBSET_DEF, domain_lookup]
-      )
-      >> asm_rewrite_tac[] >>
-      simp[wf_insert, wf_difference, wf_union, wf_delete, lookup_delete, wf_close_spt,
-        domain_union, subspt_delete, lookup_delete] >>
-        fs[domain_union] >> metis_tac[wf_union]
+        fs[] >>
+        first_x_assum match_mp_tac >>
+        fs[wf_union, wf_difference, subspt_domain, domain_union] >>
+        fs[SUBSET_DEF] >>
+        rw[] >> fs[]
+        >- (
+            match_mp_tac wf_union >>
+            fs[] >>
+            match_mp_tac wf_spt_fold_tree >>
+            fs[wf_inter, wf_def] >>
+            fs[lookup_inter] >>
+            rw[] >> EVERY_CASE_TAC >> fs[] >> 
+            rveq >>
+            fs[subspt_lookup] >>
+            res_tac >>
+            metis_tac[]
+            )
+        >-  metis_tac[]
+        >-  metis_tac[]        
+        >- (
+            qspecl_then [`tree`, `LN`] mp_tac domain_spt_fold_union >>
+            fs[domain_def] >>
+            impl_tac
+            >- (rw[] >> res_tac >> fs[SUBSET_DEF])
+            >- (rw[] >>
+                qspecl_then 
+                    [`inter tree (difference seen reachable)`, `tree`, `LN`] 
+                    mp_tac subspt_domain_spt_fold_union >>
+                rw[] >> fs[SUBSET_DEF] >>  
+                first_x_assum mp_tac >> impl_tac >> fs[] >> 
+                fs[subspt_alt, lookup_inter, domain_difference] >> rw[] >> 
+                EVERY_CASE_TAC >> fs[])
+            )
+        >- (
+            fs[domain_lookup] >>
+            imp_res_tac lookup_spt_fold_union >>
+            fs[lookup_def] >> 
+            fs[lookup_inter] >>
+            EVERY_CASE_TAC >> fs[] >>
+            rveq >>
+            fs[lookup_difference] >> EVERY_CASE_TAC >> fs[] >>
+            res_tac >>
+            qexists_tac `v'` >> fs[]
+            )
+        >- (
+            fs[domain_lookup] >>
+            imp_res_tac lookup_spt_fold_union >>
+            fs[lookup_def] >> 
+            fs[lookup_inter] >>
+            EVERY_CASE_TAC >> fs[] >>
+            rveq >>
+            fs[lookup_difference] >> EVERY_CASE_TAC >> fs[] >>
+            res_tac >>
+            qexists_tac `n` >> fs[] >>
+            fs[isReachable_def] >>
+            simp[Once RTC_CASES2] >>
+            DISJ2_TAC >>
+            qexists_tac `n1` >> fs[] >>
+            fs[isAdjacent_def]
+            )
+        >-  metis_tac[]
+        >- (
+            Cases_on `a ∈ domain seen` >> fs[] >>
+            Cases_on `a ∈ domain reachable` >> rfs[]
+            >-  metis_tac[] 
+            >>  `a ∈ domain tree` by fs[isAdjacent_def, domain_lookup] >>
+                `k ∈ domain tree` by fs[isAdjacent_def, domain_lookup] >>
+                `k ∈ domain (inter tree (difference seen reachable))` by 
+                    fs[domain_inter, domain_difference] >>
+                fs[isAdjacent_def] >>
+                fs[domain_lookup] >>
+                qspecl_then 
+                    [`inter tree (difference seen reachable)`, `LN`, `a`] 
+                    mp_tac (GSYM lookup_spt_fold_union_STRONG) >>
+                fs[lookup_def] >> strip_tac >>
+                fs[lookup_inter] >> EVERY_CASE_TAC >> fs[] >>
+                rveq >> fs[] >>
+                fs[EQ_IMP_THM] >>
+                first_x_assum match_mp_tac >>
+                fs[lookup_difference] >>
+                qexists_tac `k` >> fs[]
+            ) 
+    )
 );
 
 (**************************************** CLOSURE_SPT ****************************************)
 
 val closure_spt_lemma =
-    close_spt_thm |> Q.SPECL [`LN`, `start:num_set`, `tree`, `tree`]
+    close_spt_thm |> Q.SPECL [`LN`, `start:num_set`, `tree`]
         |> SIMP_RULE std_ss [
-            GSYM closure_spt_def, wf_def, wf_insert, subspt_def, domain_def, NOT_IN_EMPTY,
+            GSYM closure_spt_def, wf_def, wf_insert, 
+            subspt_def, domain_def, NOT_IN_EMPTY,
             domain_insert, SUBSET_DEF
            ]
         |> Q.SPECL[`domain (start:num_set)`]
         |> SIMP_RULE std_ss [
-                ConseqConvTheory.AND_CLAUSES_XX, ConseqConvTheory.IMP_CLAUSES_XX,
+                ConseqConvTheory.AND_CLAUSES_XX, 
+                ConseqConvTheory.IMP_CLAUSES_XX,
                 IN_SING, Once isReachable_def, RTC_REFL, AND_CLAUSES
            ] |> GEN_ALL
 ;
 
 val closure_spt_thm = Q.store_thm("closure_spt_thm",
-    `∀ tree start . wf start ∧ (wf_set_tree tree) ∧ (domain start ⊆ domain tree)
-    ⇒ domain (closure_spt start tree) =
+    `∀ tree start . wf start ∧ (wf_set_tree tree) ∧ 
+    (domain start ⊆ domain tree)
+  ⇒ domain (closure_spt start tree) =
         {a | ∃ n . isReachable tree n a ∧ n ∈ domain start}`,
     rw[] >> assume_tac closure_spt_lemma >> rw[] >> fs[wf_set_tree_def] >>
     first_x_assum match_mp_tac >> reverse(rw[]) >> res_tac >> fs[SUBSET_DEF] >>
     qexists_tac `k` >> fs[]
 );
-
-
-
 
 val _ = export_theory();
